fix

Foundation/Modal/Kripke/Logic/K4.lean
@@ -9,31 +9,39 @@ namespace LO.Modal
 open Kripke
 open Hilbert.Kripke
 
-protected abbrev Kripke.FrameClass.trans : FrameClass := { F | F.IsTransitive }
-protected abbrev Kripke.FrameClass.finite_trans : FrameClass := { F | F.IsFinite ∧ F.IsTransitive }
+namespace Kripke
+
+abbrev Frame.IsK4 (F : Frame) := F.IsTransitive
+class Frame.IsFiniteK4 (F : Frame) extends Frame.IsK4 F, Frame.IsFinite F
+
+protected abbrev FrameClass.K4 : FrameClass := { F | F.IsK4 }
+protected abbrev FrameClass.finite_K4 : FrameClass := { F | F.IsFiniteK4 }
+
+end Kripke
+
 
 namespace Hilbert.K4.Kripke
 
-instance sound : Sound (Hilbert.K4) Kripke.FrameClass.trans := instSound_of_validates_axioms $ by
+instance sound : Sound (Hilbert.K4) FrameClass.K4 := instSound_of_validates_axioms $ by
   apply FrameClass.Validates.withAxiomK;
   rintro F F_trans φ rfl;
   apply validate_AxiomFour_of_transitive (trans := F_trans);
 
 instance consistent : Entailment.Consistent (Hilbert.K4) :=
-  consistent_of_sound_frameclass FrameClass.trans $ by
+  consistent_of_sound_frameclass FrameClass.K4 $ by
     use whitepoint;
     apply Set.mem_setOf_eq.mpr;
     infer_instance;
 
-instance canonical : Canonical (Hilbert.K4) Kripke.FrameClass.trans := ⟨by
+instance canonical : Canonical (Hilbert.K4) FrameClass.K4 := ⟨by
   apply Set.mem_setOf_eq.mpr;
   infer_instance;
 ⟩
 
-instance complete : Complete (Hilbert.K4) Kripke.FrameClass.trans := inferInstance
+instance complete : Complete (Hilbert.K4) FrameClass.K4 := inferInstance
 
 open finestFiltrationTransitiveClosureModel in
-instance finite_complete : Complete (Hilbert.K4) Kripke.FrameClass.finite_trans := ⟨by
+instance finite_complete : Complete (Hilbert.K4) FrameClass.finite_K4 := ⟨by
   intro φ hp;
   apply Kripke.complete.complete;
   intro F F_trans V x;
@@ -42,9 +50,13 @@ instance finite_complete : Complete (Hilbert.K4) Kripke.FrameClass.finite_trans 
   let FM := finestFiltrationTransitiveClosureModel M φ.subformulas;
   apply filtration FM (finestFiltrationTransitiveClosureModel.filterOf) (by subformula) |>.mpr;
   apply hp;
+  apply Set.mem_setOf_eq.mpr;
+  sorry;
+  /-
   refine ⟨?_, ?_⟩;
   . apply finestFiltrationTransitiveClosureModel.isFinite $ by simp;
   . apply isTransitive;
+  -/
 ⟩
 
 end Hilbert.K4.Kripke
@@ -55,7 +67,7 @@ open Formula
 open Entailment
 open Kripke
 
-lemma K4.Kripke.trans : Logic.K4 = FrameClass.trans.logic := eq_hilbert_logic_frameClass_logic
+lemma K4.Kripke.trans : Logic.K4 = FrameClass.K4.logic := eq_hilbert_logic_frameClass_logic
 
 theorem K4.proper_extension_of_K : Logic.K ⊂ Logic.K4 := by
   constructor;
