Foundation/Modal/Kripke/Logic/K4M.lean
@@ -24,13 +24,9 @@ instance Kripke.sound : Sound (Hilbert.K4M) FrameClass.K4M := instSound_of_valid
 
 instance Kripke.consistent : Entailment.Consistent (Hilbert.K4M) := consistent_of_sound_frameclass FrameClass.K4M $ by
   use whitepoint;
-  apply Set.mem_setOf_eq.mpr;
   constructor;
 
-instance Kripke.canonical : Canonical (Hilbert.K4M) FrameClass.K4M := ⟨by
-  apply Set.mem_setOf_eq.mpr;
-  constructor;
-⟩
+instance Kripke.canonical : Canonical (Hilbert.K4M) FrameClass.K4M := ⟨by constructor⟩
 
 instance Kripke.complete : Complete (Hilbert.K4M) FrameClass.K4M := inferInstance
 
@@ -47,7 +43,7 @@ lemma K4M.Kripke.trans_mckinsey : Logic.K4M = FrameClass.K4M.logic := eq_hilbert
 theorem K4M.proper_extension_of_K4 : Logic.K4 ⊂ Logic.K4M := by
   constructor;
   . exact Hilbert.weakerThan_of_dominate_axioms (by simp) |>.subset;
-  . suffices ∃ φ, Hilbert.K4M ⊢! φ ∧ ¬Kripke.FrameClass.trans ⊧ φ by
+  . suffices ∃ φ, Hilbert.K4M ⊢! φ ∧ ¬FrameClass.K4 ⊧ φ by
       rw [K4.Kripke.trans];
       tauto;
     use (Axioms.M (.atom 0));
